src/SlotsAlloc.fsti
@@ -1,0 +1,44 @@
+module SlotsAlloc
+
+module U8 = FStar.UInt8
+module U32 = FStar.UInt32
+module U64 = FStar.UInt64
+
+open Steel.Effect.Atomic
+open Steel.Effect
+module A = Steel.Array
+
+open Constants
+open Utils2
+
+open SlotsCommon
+
+val allocate_slot
+  (size_class: sc)
+  (arr: array U8.t{A.length arr = U32.v page_size})
+  (md md_q: slab_metadata)
+  : Steel (array U8.t)
+  (slab_vprop size_class arr md md_q)
+  (fun r -> A.varray r `star` slab_vprop size_class arr md md_q)
+  (requires fun h0 ->
+    let blob0 : t_of (slab_vprop size_class arr md md_q)
+      = h0 (slab_vprop size_class arr md md_q) in
+    let vs0 : _ & Seq.lseq U64.t 4 = dfst (fst blob0) in
+    let v_or0 : Seq.lseq U64.t 4 = seq_u64_or (fst vs0) (snd vs0) in
+    has_free_slot size_class v_or0)
+  (ensures fun h0 r h1 ->
+    let blob0 : t_of (slab_vprop size_class arr md md_q)
+      = h0 (slab_vprop size_class arr md md_q) in
+    let blob1 : t_of (slab_vprop size_class arr md md_q)
+      = h1 (slab_vprop size_class arr md md_q) in
+    let vs0 : _ & Seq.lseq U64.t 4 = dfst (fst blob0) in
+    let vs1 : _ & Seq.lseq U64.t 4 = dfst (fst blob1) in
+    let v_or0 : Seq.lseq U64.t 4 = seq_u64_or (fst vs0) (snd vs0) in
+    let v_or1 : Seq.lseq U64.t 4 = seq_u64_or (fst vs1) (snd vs1) in
+    not (is_empty size_class v_or1) /\
+    A.length r == U32.v size_class /\
+    same_base_array r arr /\
+    A.offset (A.ptr_of r) - A.offset (A.ptr_of arr) >= 0 /\
+    A.offset (A.ptr_of r) - A.offset (A.ptr_of arr) < U32.v page_size /\
+    (A.offset (A.ptr_of r) - A.offset (A.ptr_of arr)) % (U32.v size_class) == 0
+  )
