src/SlotsFree.fsti
@@ -1,0 +1,54 @@
+module SlotsFree
+
+module U8 = FStar.UInt8
+module U32 = FStar.UInt32
+module U64 = FStar.UInt64
+module US = FStar.SizeT
+
+open Steel.Effect.Atomic
+open Steel.Effect
+module A = Steel.Array
+
+open Constants
+open Utils2
+
+open SlotsCommon
+
+
+val deallocate_slot
+  (size_class: sc)
+  (md md_q: slab_metadata)
+  (arr: array U8.t{A.length arr = U32.v page_size})
+  (ptr: array U8.t)
+  (diff_: US.t)
+  : Steel bool
+  (A.varray ptr `star` slab_vprop size_class arr md md_q)
+  (fun b ->
+    (if b then emp else A.varray ptr) `star`
+    slab_vprop size_class arr md md_q)
+  (requires fun h0 ->
+    let diff = A.offset (A.ptr_of ptr) - A.offset (A.ptr_of arr) in
+    //TODO: improve spec
+    //let blob0 : t_of (slab_vprop size_class arr md))
+    //  = h0 (slab_vprop size_class arr md) in
+    //let v0 : Seq.lseq U64.t 4 = dfst blob0 in
+    //not (is_empty size_class v0))
+    same_base_array arr ptr /\
+    0 <= diff /\
+    diff < U32.v page_size /\
+    diff % U32.v size_class == 0 /\
+    US.v diff_ = diff /\
+    A.length ptr == U32.v size_class
+  )
+  (ensures fun h0 b h1 ->
+    //TODO: improve spec
+    //let blob0 : t_of (slab_vprop size_class arr md md_q)
+    //  = h0 (slab_vprop size_class arr md md_q) in
+    //let v0 : _ & Seq.lseq U64.t 4 = dfst (fst blob0) in
+    //let blob1 : t_of (slab_vprop size_class arr md md_q)
+    //  = h1 (slab_vprop size_class arr md md_q) in
+    //let v1 : _ & Seq.lseq U64.t 4 = dfst (fst blob1) in
+    //(b ==> not (is_full size_class (fst v1))) /\
+    True
+    //(not b ==> v1 == v0)
+  )
